src/certigrad/compute_grad_slow_correct.lean
@@ -9,6 +9,7 @@ is correct.
 import .graph .estimators .predicates .compute_grad .lemmas .tgrads .tactics .is_gdifferentiable
 
 namespace certigrad
+namespace theorems
 open list
 
 lemma compute_grad_slow_correct {costs : list ID} :
@@ -432,4 +433,5 @@ apply congr_arg,
 -- 6. Apply map_filter_congr
 exact map_filter_expand_helper _ _ _ _ _ _ H_wf H_gs_exist _
 end
+end theorems
 end certigrad
